Computability/Constructions/List.lean
@@ -17,7 +17,9 @@ instance : Coe (List ℕ) ℕ := ⟨l2n⟩
 section list_nil
 namespace Nat.RecursiveIn.Code
 def c_list_nil := zero
-@[simp] theorem c_list_nil_ev_pr:code_prim c_list_nil := by repeat (first|assumption|simp|constructor)
+@[cp] theorem c_list_nil_ev_pr : code_prim c_list_nil := by
+  unfold c_list_nil
+  apply_rules (config := {maxDepth:=30, symm:=false, exfalso:=false, transparency:=.reducible}) only [*] using cp
 @[simp] theorem c_list_nil_evp :eval_prim O c_list_nil x = l2n ([]) := by simp [c_list_nil]
 @[simp] theorem c_list_nil_ev :eval O c_list_nil x = l2n ([]) := by simp [←eval_prim_eq_eval c_list_nil_ev_pr]
 end Nat.RecursiveIn.Code
@@ -26,7 +28,9 @@ end list_nil
 section list_cons
 namespace Nat.RecursiveIn.Code
 def c_list_cons := succ
-@[simp] theorem c_list_cons_ev_pr:code_prim c_list_cons := by repeat (first|assumption|simp|constructor)
+@[cp] theorem c_list_cons_ev_pr : code_prim c_list_cons := by
+  unfold c_list_cons
+  apply_rules (config := {maxDepth:=30, symm:=false, exfalso:=false, transparency:=.reducible}) only [*] using cp
 @[simp] theorem c_list_cons_evp :eval_prim O c_list_cons (Nat.pair a lN)= l2n (List.cons a (n2l lN)) := by simp [c_list_cons]
 @[simp] theorem c_list_cons_ev :eval O c_list_cons (Nat.pair a lN)= l2n (List.cons a (n2l lN)) := by simp [←eval_prim_eq_eval c_list_cons_ev_pr]
 end Nat.RecursiveIn.Code
@@ -35,7 +39,9 @@ end list_cons
 section list_tail
 namespace Nat.RecursiveIn.Code
 def c_list_tail := right.comp c_pred
-@[simp] theorem c_list_tail_ev_pr:code_prim c_list_tail := by repeat (first|assumption|simp|constructor)
+@[cp] theorem c_list_tail_ev_pr : code_prim c_list_tail := by
+  unfold c_list_tail
+  apply_rules (config := {maxDepth:=30, symm:=false, exfalso:=false, transparency:=.reducible}) only [*] using cp
 @[simp] theorem c_list_tail_evp : eval_prim O c_list_tail lN = l2n (List.tail (n2l lN)) := by
   simp [c_list_tail]
   by_cases hl:lN=0
@@ -48,7 +54,9 @@ end list_tail
 section list_head?
 namespace Nat.RecursiveIn.Code
 def c_list_head? := c_ifz.comp₃ c_id zero $ succ.comp (left.comp c_pred)
-@[simp] theorem c_list_head?_ev_pr:code_prim c_list_head? := by repeat (first|assumption|simp|constructor)
+@[cp] theorem c_list_head?_ev_pr : code_prim c_list_head? := by
+  unfold c_list_head?
+  apply_rules (config := {maxDepth:=30, symm:=false, exfalso:=false, transparency:=.reducible}) only [*] using cp
 @[simp] theorem c_list_head?_evp : eval_prim O c_list_head? lN = o2n (List.head? (n2l lN)) := by
   simp [c_list_head?]
   by_cases hl:lN=0
@@ -63,7 +71,9 @@ end list_head?
 section list_headI
 namespace Nat.RecursiveIn.Code
 def c_list_headI := c_ifz.comp₃ c_id zero (left.comp c_pred)
-@[simp] theorem c_list_headI_ev_pr:code_prim c_list_headI := by repeat (first|assumption|simp|constructor)
+@[cp] theorem c_list_headI_ev_pr : code_prim c_list_headI := by
+  unfold c_list_headI
+  apply_rules (config := {maxDepth:=30, symm:=false, exfalso:=false, transparency:=.reducible}) only [*] using cp
 @[simp] theorem c_list_headI_evp : eval_prim O c_list_headI lN = List.headI (n2l lN) := by
   simp [c_list_headI]
   by_cases hl:lN=0
@@ -79,7 +89,9 @@ def c_list_casesOn (cl cf cg:Code) :=
   let x := left.comp (c_pred.comp cl)
   let xs := right.comp (c_pred.comp cl)
   c_if_eq_te.comp₄ cl (c_const 0) cf (cg.comp₂ x xs)
-@[simp] theorem c_list_casesOn_ev_pr (hcl:code_prim cl) (hcf:code_prim cf) (hcg:code_prim cg):code_prim (c_list_casesOn cl cf cg) := by repeat (first|assumption|simp|constructor)
+@[cp] theorem c_list_casesOn_ev_pr (hcl:code_prim cl) (hcf:code_prim cf) (hcg:code_prim cg) : code_prim (c_list_casesOn cl cf cg) := by
+  unfold c_list_casesOn
+  apply_rules (config := {maxDepth:=30, symm:=false, exfalso:=false, transparency:=.reducible}) only [*] using cp
 @[simp] theorem c_list_casesOn_evp : eval_prim O (c_list_casesOn cl cf cg) input =
   List.casesOn
   (n2l (eval_prim O cl input))
@@ -102,7 +114,9 @@ section list_casesOn'
 namespace Nat.RecursiveIn.Code
 def c_list_casesOn' (cl cf cg:Code) :=
   c_if_eq_te.comp₄ cl (c_const 0) cf cg
-@[simp] theorem c_list_casesOn'_ev_pr (hcl:code_prim cl) (hcf:code_prim cf) (hcg:code_prim cg):code_prim (c_list_casesOn' cl cf cg) := by repeat (first|assumption|simp|constructor)
+@[cp] theorem c_list_casesOn'_ev_pr (hcl:code_prim cl) (hcf:code_prim cf) (hcg:code_prim cg):code_prim (c_list_casesOn' cl cf cg) := by
+  unfold c_list_casesOn'
+  apply_rules (config := {maxDepth:=30, symm:=false, exfalso:=false, transparency:=.reducible}) only [*] using cp
 @[simp] theorem c_list_casesOn'_evp : eval_prim O (c_list_casesOn' cl cf cg) input =
   List.casesOn
   (n2l (eval_prim O cl input))
@@ -130,7 +144,9 @@ def c_list_drop :=
     c_id $
     c_list_tail.comp (right.comp right)
   ).comp c_flip
-@[simp] theorem c_list_drop_ev_pr:code_prim c_list_drop := by repeat (first|assumption|simp|constructor)
+@[cp] theorem c_list_drop_ev_pr : code_prim c_list_drop := by
+  unfold c_list_drop
+  apply_rules (config := {maxDepth:=30, symm:=false, exfalso:=false, transparency:=.reducible}) only [*] using cp
 @[simp] theorem c_list_drop_evp : eval_prim O c_list_drop (Nat.pair i lN) = l2n (List.drop i (n2l lN)) := by
   simp [c_list_drop]
   by_cases hl:lN=0
@@ -149,7 +165,9 @@ end list_drop
 section list_getElem?
 namespace Nat.RecursiveIn.Code
 def c_list_getElem? := c_list_head?.comp (c_list_drop.comp c_flip)
-@[simp] theorem c_list_getElem?_ev_pr:code_prim c_list_getElem? := by repeat (first|assumption|simp|constructor)
+@[cp] theorem c_list_getElem?_ev_pr : code_prim c_list_getElem? := by
+  unfold c_list_getElem?
+  apply_rules (config := {maxDepth:=30, symm:=false, exfalso:=false, transparency:=.reducible}) only [*] using cp
 @[simp] theorem c_list_getElem?_evp : eval_prim O c_list_getElem? (Nat.pair lN i) = o2n (n2l lN)[i]? := by simp [c_list_getElem?]
 @[simp] theorem c_list_getElem?_ev : eval O c_list_getElem? (Nat.pair lN i) = o2n (n2l lN)[i]? := by simp [← eval_prim_eq_eval c_list_getElem?_ev_pr]
 end Nat.RecursiveIn.Code
@@ -158,7 +176,9 @@ end list_getElem?
 section list_getD
 namespace Nat.RecursiveIn.Code
 def c_list_getD := c_opt_getD.comp₂ (c_list_getElem?.comp₂ left (left.comp right)) (right.comp right)
-@[simp] theorem c_list_getD_ev_pr:code_prim c_list_getD := by repeat (first|assumption|simp|constructor)
+@[cp] theorem c_list_getD_ev_pr : code_prim c_list_getD := by
+  unfold c_list_getD
+  apply_rules (config := {maxDepth:=30, symm:=false, exfalso:=false, transparency:=.reducible}) only [*] using cp
 @[simp] theorem c_list_getD_evp : eval_prim O c_list_getD (Nat.pair lN (Nat.pair i d)) = (n2l lN).getD i d := by simp [c_list_getD]
 @[simp] theorem c_list_getD_ev : eval O c_list_getD (Nat.pair lN (Nat.pair i d)) = (n2l lN).getD i d := by simp [← eval_prim_eq_eval c_list_getD_ev_pr]
 end Nat.RecursiveIn.Code
@@ -167,7 +187,9 @@ end list_getD
 section list_getI
 namespace Nat.RecursiveIn.Code
 def c_list_getI := c_pred.comp c_list_getElem?
-@[simp] theorem c_list_getI_ev_pr:code_prim c_list_getI := by repeat (first|assumption|simp|constructor)
+@[cp] theorem c_list_getI_ev_pr : code_prim c_list_getI := by
+  unfold c_list_getI
+  apply_rules (config := {maxDepth:=30, symm:=false, exfalso:=false, transparency:=.reducible}) only [*] using cp
 @[simp] theorem c_list_getI_evp : eval_prim O c_list_getI (Nat.pair lN i) = ((n2l lN).getI i) := by
   simp [c_list_getI]
   by_cases hl:i<(n2l lN).length <;> simp [hl, List.getI]
@@ -178,7 +200,9 @@ end list_getI
 section list_get
 namespace Nat.RecursiveIn.Code
 def c_list_get := c_list_getI
-@[simp] theorem c_list_get_ev_pr:code_prim c_list_get := by repeat (first|assumption|simp|constructor)
+@[cp] theorem c_list_get_ev_pr : code_prim c_list_get := by
+  unfold c_list_get
+  apply_rules (config := {maxDepth:=30, symm:=false, exfalso:=false, transparency:=.reducible}) only [*] using cp
 @[simp] theorem c_list_get_evp (h:i<(n2l lN).length) : eval_prim O c_list_get (Nat.pair lN i) = (n2l lN)[i] := by
   simp [c_list_get]
   simp [getI]
@@ -204,7 +228,9 @@ def c_list_foldl_aux (cf:Code) :=
   c_list_casesOn' right c_id (pair (cf.comp₂ left x) (xs))
 def c_list_foldl_aux2 (cf:Code) := (c_nat_iterate (c_list_foldl_aux cf)).comp₂ c_id right
 def c_list_foldl (cf:Code) := left.comp (c_list_foldl_aux2 cf)
-@[simp] theorem c_list_foldl_ev_pr(hcf:code_prim cf):code_prim (c_list_foldl cf) := by repeat (first|assumption|simp|constructor)
+@[cp] theorem c_list_foldl_ev_pr (hcf:code_prim cf) : code_prim (c_list_foldl cf) := by
+  rewrite [c_list_foldl, c_list_foldl_aux2, c_list_foldl_aux]
+  apply_rules (config := {maxDepth:=30, symm:=false, exfalso:=false, transparency:=.reducible}) only [*] using cp
 @[simp] theorem c_list_foldl_aux_evp   : eval_prim O (c_list_foldl_aux cf) (Nat.pair init lN) = if (n2l lN) = [] then (Nat.pair init lN) else Nat.pair (eval_prim O cf (Nat.pair init (n2l lN).headI)) (l2n (List.tail (n2l lN))) := by
   simp [c_list_foldl_aux]
   by_cases hl:lN=0
@@ -285,7 +311,9 @@ end list_foldl
 section list_reverse
 namespace Nat.RecursiveIn.Code
 def c_list_reverse := (c_list_foldl (c_list_cons.comp c_flip)).comp₂ c_list_nil c_id
-@[simp] theorem c_list_reverse_ev_pr:code_prim c_list_reverse := by repeat (first|assumption|simp|constructor)
+@[cp] theorem c_list_reverse_ev_pr : code_prim c_list_reverse := by
+  unfold c_list_reverse
+  apply_rules (config := {maxDepth:=30, symm:=false, exfalso:=false, transparency:=.reducible}) only [*] using cp
 @[simp] theorem c_list_reverse_evp : eval_prim O c_list_reverse lN =  l2n (List.reverse (n2l lN)) := by
   simp only [c_list_reverse]
   simp [-encode_list_cons, -encode_list_nil]
@@ -308,7 +336,9 @@ end list_reverse
 section list_foldr
 namespace Nat.RecursiveIn.Code
 def c_list_foldr (cf:Code) := (c_list_foldl (cf.comp c_flip)).comp₂ left (c_list_reverse.comp right)
-@[simp] theorem c_list_foldr_ev_pr(hcf:code_prim cf):code_prim (c_list_foldr cf) := by repeat (first|assumption|simp|constructor)
+@[cp] theorem c_list_foldr_ev_pr(hcf:code_prim cf) : code_prim (c_list_foldr cf) := by
+  unfold c_list_foldr
+  apply_rules (config := {maxDepth:=30, symm:=false, exfalso:=false, transparency:=.reducible}) only [*] using cp
 @[simp] theorem c_list_foldr_evp : eval_prim O (c_list_foldr cf) (Nat.pair init lN) =
   (
     List.foldr
@@ -331,7 +361,9 @@ end list_foldr
 section list_length
 namespace Nat.RecursiveIn.Code
 def c_list_length := (c_list_foldl (succ.comp left)).comp₂ zero c_id
-@[simp] theorem c_list_length_ev_pr:code_prim c_list_length := by repeat (first|assumption|simp|constructor)
+@[cp] theorem c_list_length_ev_pr : code_prim c_list_length := by
+  unfold c_list_length
+  apply_rules (config := {maxDepth:=30, symm:=false, exfalso:=false, transparency:=.reducible}) only [*] using cp
 @[simp] theorem c_list_length_evp : eval_prim O c_list_length lN = List.length (n2l lN) := by simp [c_list_length]
 @[simp] theorem c_list_length_ev : eval O c_list_length lN = List.length (n2l lN) := by simp [← eval_prim_eq_eval c_list_length_ev_pr]
 end Nat.RecursiveIn.Code
@@ -340,7 +372,9 @@ end list_length
 section list_getLast?
 namespace Nat.RecursiveIn.Code
 def c_list_getLast? := c_list_getElem?.comp₂ c_id (c_pred.comp $ c_list_length.comp c_id)
-@[simp] theorem c_list_getLast?_ev_pr:code_prim c_list_getLast? := by repeat (first|assumption|simp|constructor)
+@[cp] theorem c_list_getLast?_ev_pr : code_prim c_list_getLast? := by
+  unfold c_list_getLast?
+  apply_rules (config := {maxDepth:=30, symm:=false, exfalso:=false, transparency:=.reducible}) only [*] using cp
 @[simp] theorem c_list_getLast?_evp : eval_prim O c_list_getLast? lN = o2n (List.getLast? (n2l lN)) := by
   simp [c_list_getLast?]
   exact Eq.symm List.getLast?_eq_getElem?
@@ -351,7 +385,9 @@ end list_getLast?
 section list_getLastI
 namespace Nat.RecursiveIn.Code
 def c_list_getLastI := c_opt_iget.comp c_list_getLast?
-@[simp] theorem c_list_getLastI_ev_pr:code_prim c_list_getLastI := by repeat (first|assumption|simp|constructor)
+@[cp] theorem c_list_getLastI_ev_pr : code_prim c_list_getLastI := by
+  unfold c_list_getLastI
+  apply_rules (config := {maxDepth:=30, symm:=false, exfalso:=false, transparency:=.reducible}) only [*] using cp
 @[simp] theorem c_list_getLastI_evp : eval_prim O c_list_getLastI lN = List.getLastI (n2l lN) := by
   simp [c_list_getLastI]
   exact Eq.symm (List.getLastI_eq_getLast? (n2l lN))
@@ -366,7 +402,9 @@ end list_getLastI
 section list_append
 namespace Nat.RecursiveIn.Code
 def c_list_append := (c_list_foldr (c_list_cons)).comp c_flip
-@[simp] theorem c_list_append_ev_pr:code_prim c_list_append := by repeat (first|assumption|simp|constructor)
+@[cp] theorem c_list_append_ev_pr : code_prim c_list_append := by
+  unfold c_list_append
+  apply_rules (config := {maxDepth:=30, symm:=false, exfalso:=false, transparency:=.reducible}) only [*] using cp
 @[simp] theorem c_list_append_evp : eval_prim O c_list_append (Nat.pair l1N l2N) = l2n ((n2l l1N) ++ (n2l l2N)) := by
   simp [c_list_append, -encode_list_cons, -encode_list_nil]
   induction (n2l l1N) with
@@ -379,7 +417,9 @@ end list_append
 section list_singleton
 namespace Nat.RecursiveIn.Code
 def c_list_singleton (cf:Code) := c_list_cons.comp₂ cf c_list_nil
-@[simp] theorem c_list_singleton_ev_pr :code_prim (c_list_singleton c_flip) := by repeat (first|assumption|simp|constructor)
+@[cp] theorem c_list_singleton_ev_pr (hcf:code_prim cf) : code_prim (c_list_singleton cf) := by
+  unfold c_list_singleton
+  apply_rules (config := {maxDepth:=30, symm:=false, exfalso:=false, transparency:=.reducible}) only [*] using cp
 @[simp] theorem c_list_singleton_evp : eval_prim O (c_list_singleton cf) x = l2n ([eval_prim O cf x]) := by
   simp [c_list_singleton]
 -- @[simp] theorem c_list_singleton_ev : eval O (c_list_singleton cf) x = l2n ([eval_prim O cf x]) := by simp [← eval_prim_eq_eval c_list_singleton_ev_pr]
@@ -389,7 +429,9 @@ end list_singleton
 section list_concat
 namespace Nat.RecursiveIn.Code
 def c_list_concat := c_list_append.comp₂ left (c_list_singleton right)
-@[simp] theorem c_list_concat_ev_pr:code_prim c_list_concat := by repeat (first|assumption|simp|constructor)
+@[cp] theorem c_list_concat_ev_pr : code_prim c_list_concat := by
+  unfold c_list_concat
+  apply_rules (config := {maxDepth:=30, symm:=false, exfalso:=false, transparency:=.reducible}) only [*] using cp
 @[simp] theorem c_list_concat_evp : eval_prim O c_list_concat (Nat.pair lN i) = l2n ((n2l lN)++[i]) := by
   simp [c_list_concat, -encode_list_cons, -encode_list_nil]
 @[simp] theorem c_list_concat_ev : eval O c_list_concat (Nat.pair lN i) = l2n ((n2l lN)++[i]) := by simp [← eval_prim_eq_eval c_list_concat_ev_pr]
@@ -400,7 +442,9 @@ end list_concat
 section list_map
 namespace Nat.RecursiveIn.Code
 def c_list_map (cf:Code) := (c_list_foldr (c_list_cons.comp₂ (cf.comp left) right)).comp₂ (c_list_nil) (c_id)
-@[simp] theorem c_list_map_ev_pr (hcf:code_prim cf): code_prim (c_list_map cf) := by repeat (first|assumption|simp|constructor)
+@[cp] theorem c_list_map_ev_pr (hcf:code_prim cf) : code_prim (c_list_map cf) := by
+  unfold c_list_map
+  apply_rules (config := {maxDepth:=30, symm:=false, exfalso:=false, transparency:=.reducible}) only [*] using cp
 @[simp] theorem c_list_map_evp : eval_prim O (c_list_map cf) lN = l2n ((n2l lN).map (eval_prim O cf)) := by
   simp [c_list_map, -encode_list_cons, -encode_list_nil]
   induction (n2l lN) with
@@ -436,7 +480,12 @@ def c_list_zipWith_aux (cf:Code):=
 def c_list_zipWith (cf:Code) := c_list_reverse.comp $ left.comp (c_list_zipWith_aux cf)
 -- #eval eval_prim (Nat.fzero) c_list_zipWith_aux (Nat.pair [1] [3])
 -- theorem zip_aux : List.foldr () = List.zip ()
-@[simp] theorem c_list_zipWith_ev_pr (hcf:code_prim cf) : code_prim (c_list_zipWith_aux cf) := by repeat (first|assumption|simp|constructor)
+@[cp] theorem c_list_zipWith_aux_ev_pr (hcf:code_prim cf) : code_prim (c_list_zipWith_aux cf) := by
+  unfold c_list_zipWith_aux
+  apply_rules (config := {maxDepth:=30, symm:=false, exfalso:=false, transparency:=.reducible}) only [*] using cp
+@[cp] theorem c_list_zipWith_ev_pr (hcf:code_prim cf) : code_prim (c_list_zipWith cf) := by
+  unfold c_list_zipWith
+  apply_rules (config := {maxDepth:=30, symm:=false, exfalso:=false, transparency:=.reducible}) only [*] using cp
 -- @[simp] theorem c_list_zipWith_evp : eval_prim O c_list_zipWith_aux (Nat.pair l1N l2N) = l2n (List.zipWith Nat.pair (n2l l1N) (n2l l2N)) := by
 theorem c_list_zipWith_evp_aux_2 {a b : List ℕ} {f:ℕ→ℕ→ℕ} (h:a.length≤b.length) : List.zipWith f (b++c) a = List.zipWith f b a := by
   have aux3 : b = take a.length (b) ++ drop a.length (b) := by
@@ -578,7 +627,9 @@ def c_list_range :=
   (prec
   (c_list_nil)
   (c_list_concat.comp₂ prev_list i)).comp₂ zero c_id
-@[simp] theorem c_list_range_ev_pr : code_prim c_list_range := by repeat (first|assumption|simp|constructor)
+@[cp] theorem c_list_range_ev_pr : code_prim c_list_range := by
+  unfold c_list_range
+  apply_rules (config := {maxDepth:=30, symm:=false, exfalso:=false, transparency:=.reducible}) only [*] using cp
 @[simp] theorem c_list_range_evp : eval_prim O c_list_range n = l2n (List.range n) := by
   simp [c_list_range, -encode_list_cons, -encode_list_nil]
   induction n with
@@ -598,7 +649,9 @@ def c_list_replicate :=
   (prec
   (c_list_nil)
   (c_list_concat.comp₂ prev_list x)).comp c_flip
-@[simp] theorem c_list_replicate_ev_pr : code_prim c_list_replicate := by repeat (first|assumption|simp|constructor)
+@[cp] theorem c_list_replicate_ev_pr : code_prim c_list_replicate := by
+  unfold c_list_replicate
+  apply_rules (config := {maxDepth:=30, symm:=false, exfalso:=false, transparency:=.reducible}) only [*] using cp
 @[simp] theorem c_list_replicate_evp : eval_prim O c_list_replicate (Nat.pair n x) = l2n (List.replicate n x) := by
   simp [c_list_replicate, -encode_list_cons, -encode_list_nil]
   induction n with
@@ -619,7 +672,10 @@ def c_list_map' (cf:Code) :=
   let lN  := left
   let aux := right
   (c_list_map cf).comp ((c_list_zipWith c_id).comp₂ lN (c_list_replicate.comp₂ (c_list_length.comp lN) aux))
-@[simp, aesop safe] theorem c_list_map'_ev_pr (hcf:code_prim cf): code_prim (c_list_map' cf) := by repeat (first|assumption|simp|constructor)
+@[cp] theorem c_list_map'_ev_pr (hcf:code_prim cf) : code_prim (c_list_map' cf) := by
+  unfold c_list_map'
+  apply_rules (config := {maxDepth:=30, symm:=false, exfalso:=false, transparency:=.reducible}) only [*] using cp
+
 @[simp] theorem c_list_map'_evp :
   eval_prim O (c_list_map' cf) (Nat.pair lN aux)
     =
