Computability/Constructions/Primitive.lean
@@ -5,7 +5,9 @@ open Nat.RecursiveIn.Code
 section comp₂
 namespace Nat.RecursiveIn.Code
 def comp₂ : Code→Code→Code→Code := fun c1 c2 c3 => c1.comp (pair c2 c3)
-@[simp, aesop safe] theorem comp₂_ev_pr {c1 c2 c3} (hc1:code_prim c1) (hc2:code_prim c2) (hc3:code_prim c3) :code_prim (comp₂ c1 c2 c3) := by repeat (first|assumption|simp|constructor)
+@[cp] theorem comp₂_ev_pr {c1 c2 c3} (hc1:code_prim c1) (hc2:code_prim c2) (hc3:code_prim c3) :code_prim (comp₂ c1 c2 c3) := by
+  unfold comp₂
+  apply_rules (config := {maxDepth:=30, symm:=false, exfalso:=false, transparency:=.reducible}) only [*] using cp
 -- theorem comp₂_evp:eval_prim O (comp₂ c1 c2 c3) x = eval_prim O c1 (Nat.pair (eval_prim O (c2) x) (eval_prim O (c3) x))  := by simp [comp₂,eval_prim];
 @[simp] theorem comp₂_evp {O c1 c2 c3}:eval_prim O (comp₂ c1 c2 c3) = fun x => eval_prim O c1 (Nat.pair (eval_prim O (c2) x) (eval_prim O (c3) x))  := by simp [comp₂,eval_prim];
 @[simp] theorem comp₂_ev {O c1 c2 c3} : eval O (comp₂ c1 c2 c3) = fun x => (Nat.pair <$> (eval O (c2) x) <*> (eval O (c3) x)) >>= (eval O c1) := by simp [eval, comp₂, Seq.seq]
@@ -16,7 +18,9 @@ end comp₂
 section comp₄
 namespace Nat.RecursiveIn.Code
 def comp₄ : Code→Code→Code→Code→Code→Code := fun c1 c2 c3 c4 c5 => c1.comp₂ (pair c2 c3) (pair c4 c5)
-@[simp, aesop safe] theorem comp₄_ev_pr {c1 c2 c3 c4 c5} (hc1:code_prim c1) (hc2:code_prim c2) (hc3:code_prim c3) (hc4:code_prim c4) (hc5:code_prim c5):code_prim (comp₄ c1 c2 c3 c4 c5) := by repeat (first|assumption|simp|constructor)
+@[cp] theorem comp₄_ev_pr {c1 c2 c3 c4 c5} (hc1:code_prim c1) (hc2:code_prim c2) (hc3:code_prim c3) (hc4:code_prim c4) (hc5:code_prim c5):code_prim (comp₄ c1 c2 c3 c4 c5) := by
+  unfold comp₄
+  apply_rules (config := {maxDepth:=30, symm:=false, exfalso:=false, transparency:=.reducible}) only [*] using cp
 @[simp] theorem comp₄_evp {O c1 c2 c3 c4 c5} : eval_prim O (comp₄ c1 c2 c3 c4 c5) = λ x ↦
   eval_prim O c1 (Nat.pair (Nat.pair (eval_prim O c2 x) (eval_prim O c3 x)) (Nat.pair (eval_prim O c4 x) (eval_prim O c5 x))) := by
   simp [comp₄,eval_prim, comp₂];
@@ -35,7 +39,9 @@ end comp₄
 section comp₃
 namespace Nat.RecursiveIn.Code
 def comp₃ : Code→Code→Code→Code→Code := fun c1 c2 c3 c4 => c1.comp₂ c2 (pair c3 c4)
-@[simp, aesop safe] theorem comp₃_ev_pr (hc1:code_prim c1) (hc2:code_prim c2) (hc3:code_prim c3) (hc4:code_prim c4) :code_prim (comp₃ c1 c2 c3 c4) := by repeat (first|assumption|simp|constructor)
+@[cp] theorem comp₃_ev_pr (hc1:code_prim c1) (hc2:code_prim c2) (hc3:code_prim c3) (hc4:code_prim c4) :code_prim (comp₃ c1 c2 c3 c4) := by
+  unfold comp₃
+  apply_rules (config := {maxDepth:=30, symm:=false, exfalso:=false, transparency:=.reducible}) only [*] using cp
 @[simp] theorem comp₃_evp:eval_prim O (comp₃ c1 c2 c3 c4) = λ x ↦
   eval_prim O c1 (Nat.pair (eval_prim O (c2) x) ((Nat.pair (eval_prim O (c3) x) (eval_prim O (c4) x)))) := by
   simp [comp₃,eval_prim]
@@ -57,7 +63,9 @@ end comp₃
 section id
 namespace Nat.RecursiveIn.Code
 def c_id := left.pair right
-@[simp, aesop safe] theorem c_id_ev_pr:code_prim c_id := by repeat (first|assumption|simp|constructor)
+@[cp] theorem c_id_ev_pr:code_prim c_id := by
+  unfold c_id
+  apply_rules (config := {maxDepth:=30, symm:=false, exfalso:=false, transparency:=.reducible}) only [*] using cp
 @[simp] theorem c_id_evp:eval_prim O c_id n= n := by simp [c_id,eval_prim]
 @[simp] theorem c_id_ev:eval O c_id n = n := by simp [c_id,eval,Seq.seq]
   -- #check @eval_prim_eq_eval c_id O c_id_ev_pr
@@ -71,7 +79,7 @@ namespace Nat.RecursiveIn.Code
 def c_const:ℕ→Code
 | 0 => zero
 | n+1 => comp succ (c_const n)
-@[simp] theorem c_const_ev_pr:code_prim (c_const n) := by
+@[cp] theorem c_const_ev_pr:code_prim (c_const n) := by
   induction n
   · unfold c_const; exact code_prim.zero
   · unfold c_const
@@ -123,7 +131,9 @@ section sgsg'
 @[simp] def Nat.sg' := fun x => if x=0 then 1 else 0
 namespace Nat.RecursiveIn.Code
 def c_sg := comp (prec zero (((c_const 1).comp left).comp left)) (pair zero c_id)
-@[simp, aesop safe] theorem c_sg_ev_pr:code_prim c_sg := by repeat (first|assumption|simp|constructor)
+@[cp] theorem c_sg_ev_pr:code_prim c_sg := by
+  unfold c_sg
+  apply_rules (config := {maxDepth:=30, symm:=false, exfalso:=false, transparency:=.reducible}) only [*] using cp
 @[simp] theorem c_sg_evp:eval_prim O c_sg = Nat.sg := by
   simp [c_sg,eval_prim]
   funext n; induction n with
@@ -131,7 +141,9 @@ def c_sg := comp (prec zero (((c_const 1).comp left).comp left)) (pair zero c_id
   | succ n _ => simp
 @[simp] theorem c_sg_ev : eval O c_sg = Nat.sg := by rw [← eval_prim_eq_eval c_sg_ev_pr]; simp only [c_sg_evp]
 def c_sg' := comp (prec (c_const 1) (((zero).comp left).comp left)) (pair zero c_id)
-@[simp, aesop safe] theorem c_sg'_ev_pr:code_prim c_sg' := by repeat (first|assumption|simp|constructor)
+@[cp] theorem c_sg'_ev_pr:code_prim c_sg' := by
+  unfold c_sg'
+  apply_rules (config := {maxDepth:=30, symm:=false, exfalso:=false, transparency:=.reducible}) only [*] using cp
 @[simp] theorem c_sg'_evp:eval_prim O c_sg' = Nat.sg' := by
   simp [c_sg',eval_prim]
   funext n; induction n with
@@ -152,7 +164,9 @@ end sgsg'
 section add
 namespace Nat.RecursiveIn.Code
 def c_add := (prec c_id ((succ.comp right).comp right))
-@[simp, aesop safe] theorem c_add_ev_pr:code_prim c_add := by repeat (first|assumption|simp|constructor)
+@[cp] theorem c_add_ev_pr:code_prim c_add := by
+  unfold c_add
+  apply_rules (config := {maxDepth:=30, symm:=false, exfalso:=false, transparency:=.reducible}) only [*] using cp
 @[simp] theorem c_add_evp:eval_prim O c_add = unpaired2 Nat.add := by
   simp [c_add,eval_prim]
   funext n;
@@ -168,7 +182,9 @@ end add
 section mul
 namespace Nat.RecursiveIn.Code
 def c_mul := prec zero (c_add.comp (pair left (right.comp right)))
-@[simp, aesop safe] theorem c_mul_ev_pr:code_prim c_mul := by repeat (first|assumption|simp|constructor)
+@[cp] theorem c_mul_ev_pr:code_prim c_mul := by
+  unfold c_mul
+  apply_rules (config := {maxDepth:=30, symm:=false, exfalso:=false, transparency:=.reducible}) only [*] using cp
 @[simp] theorem c_mul_evp:eval_prim O c_mul = unpaired2 Nat.mul := by
   simp [c_mul,eval_prim]
   funext n;
@@ -186,7 +202,9 @@ end mul
 section pow
 namespace Nat.RecursiveIn.Code
 def c_pow := prec (c_const 1) (c_mul.comp (pair (right.comp right) left))
-@[simp, aesop safe] theorem c_pow_ev_pr:code_prim c_pow := by repeat (first|assumption|simp|constructor)
+@[cp] theorem c_pow_ev_pr:code_prim c_pow := by
+  unfold c_pow
+  apply_rules (config := {maxDepth:=30, symm:=false, exfalso:=false, transparency:=.reducible}) only [*] using cp
 @[simp] theorem c_pow_evp:eval_prim O c_pow = unpaired2 Nat.pow := by
   simp [c_pow,eval_prim]
   funext n;
@@ -204,13 +222,9 @@ end pow
 section prec1
 namespace Nat.RecursiveIn.Code
 def c_prec1 (m) (cf:Code) := ((prec (c_const m) (cf.comp right)).comp (zero.pair c_id))
-@[simp] theorem c_prec1_ev_pr (hcf:code_prim cf) : code_prim (@c_prec1 m cf) := by
+@[cp] theorem c_prec1_ev_pr (hcf:code_prim cf) : code_prim (@c_prec1 m cf) := by
   unfold c_prec1;
-  repeat constructor
-  simp
-  repeat constructor
-  exact hcf
-  repeat constructor
+  apply_rules (config := {maxDepth:=30, symm:=false, exfalso:=false, transparency:=.reducible}) only [*] using cp
 @[simp] theorem c_prec1_ev : eval_prim O (c_prec1 m cf) = (fun n => n.rec m fun y IH => eval_prim O cf <| Nat.pair y IH) := by simp [c_prec1,eval_prim]
 end Nat.RecursiveIn.Code
 -- theorem Nat.PrimrecIn.prec1:Nat.PrimrecIn O Nat.prec1 := by ...
@@ -219,7 +233,9 @@ end prec1
 section casesOn1
 namespace Nat.RecursiveIn.Code
 def c_casesOn1 (m) (cf:Code) := @c_prec1 m (cf.comp left)
--- theorem c_casesOn1_ev_pr:code_prim (@c_casesOn1 a b) := by repeat constructor;
+@[cp] theorem c_casesOn1_ev_pr (hcf:code_prim cf): code_prim (c_casesOn1 m cf) := by
+  unfold c_casesOn1
+  apply_rules (config := {maxDepth:=30, symm:=false, exfalso:=false, transparency:=.reducible}) only [*] using cp
 @[simp] theorem c_casesOn1_ev : eval_prim O (@c_casesOn1 m cf) = (Nat.casesOn · m (eval_prim O cf)) := by simp [c_casesOn1,eval_prim]
 end Nat.RecursiveIn.Code
 -- theorem Nat.PrimrecIn.casesOn1:Nat.PrimrecIn O Nat.casesOn1 := by ...
@@ -229,7 +245,9 @@ end casesOn1
 section pred
 namespace Nat.RecursiveIn.Code
 def c_pred := (c_casesOn1 0 c_id)
-@[simp, aesop safe] theorem c_pred_ev_pr:code_prim c_pred := by repeat (first|assumption|simp|constructor)
+@[cp] theorem c_pred_ev_pr:code_prim c_pred := by
+  unfold c_pred
+  apply_rules (config := {maxDepth:=30, symm:=false, exfalso:=false, transparency:=.reducible}) only [*] using cp
 @[simp] theorem c_pred_evp:eval_prim O c_pred = Nat.pred := by
   simp [c_pred]
   funext n;
@@ -242,7 +260,9 @@ end pred
 section sub
 namespace Nat.RecursiveIn.Code
 def c_sub := prec c_id ((c_pred.comp right).comp right)
-@[simp, aesop safe] theorem c_sub_ev_pr:code_prim c_sub := by repeat (first|assumption|simp|constructor)
+@[cp] theorem c_sub_ev_pr:code_prim c_sub := by
+  unfold c_sub
+  apply_rules (config := {maxDepth:=30, symm:=false, exfalso:=false, transparency:=.reducible}) only [*] using cp
 @[simp] theorem c_sub_evp:eval_prim O c_sub = unpaired2 Nat.sub := by
   simp [c_sub,eval_prim]
   funext n;
@@ -259,7 +279,9 @@ end sub
 section dist
 namespace Nat.RecursiveIn.Code
 def c_dist := c_add.comp (pair c_sub (c_sub.comp (pair right left)))
-@[simp, aesop safe] theorem c_dist_ev_pr:code_prim c_dist := by repeat (first|assumption|simp|constructor)
+@[cp] theorem c_dist_ev_pr:code_prim c_dist := by
+  unfold c_dist
+  apply_rules (config := {maxDepth:=30, symm:=false, exfalso:=false, transparency:=.reducible}) only [*] using cp
 @[simp] theorem c_dist_evp:eval_prim O c_dist = unpaired2 Nat.dist := by simp [c_dist,eval_prim]; exact rfl
 @[simp] theorem c_dist_ev:eval O c_dist = unpaired2 Nat.dist := by rw [← eval_prim_eq_eval c_dist_ev_pr]; simp only [c_dist_evp]
 end Nat.RecursiveIn.Code
@@ -277,7 +299,9 @@ section if_eq'
 namespace Nat.RecursiveIn.Code
 /-- eval c_if_eq' (x,y) = [x=y] -/
 def c_if_eq' := c_sg.comp c_dist
-@[simp, aesop safe] theorem c_if_eq'_ev_pr:code_prim c_if_eq' := by repeat (first|assumption|simp|constructor)
+@[cp] theorem c_if_eq'_ev_pr:code_prim c_if_eq' := by
+  unfold c_if_eq'
+  apply_rules (config := {maxDepth:=30, symm:=false, exfalso:=false, transparency:=.reducible}) only [*] using cp
 @[simp] theorem c_if_eq'_evp:eval_prim O c_if_eq' = fun ab => if ab.l=ab.r then 0 else 1 := by simp [c_if_eq',eval_prim];
 @[simp] theorem c_if_eq'_ev:eval O c_if_eq' = fun ab => if ab.l=ab.r then Part.some 0 else Part.some 1 := by
   rw [← eval_prim_eq_eval c_if_eq'_ev_pr]; simp only [c_if_eq'_evp]; funext xs; exact apply_ite Part.some (xs.l = xs.r) 0 1
@@ -294,7 +318,14 @@ def c_if_eq_te :=
   c_add.comp₂
   (c_mul.comp₂ eq (right.comp right))
   (c_mul.comp₂ (c_not.comp eq) (left.comp right))
-@[simp, aesop safe] theorem c_if_eq_te_ev_pr:code_prim c_if_eq_te := by repeat (first|assumption|simp|constructor)
+@[cp] theorem c_if_eq_te_ev_pr:code_prim c_if_eq_te := by
+  unfold c_if_eq_te
+  extract_lets
+  expose_names
+  have cp_eq : code_prim eq := by apply_rules (config := {maxDepth:=30, symm:=false, exfalso:=false, transparency:=.reducible}) only [*] using cp
+  apply_rules (config := {maxDepth:=30, symm:=false, exfalso:=false, transparency:=.reducible}) only [*] using cp
+  -- repeat (first|assumption|simp|constructor)
+-- with the old (first|assumption|simp|constructor), this takes 245 calls.
 
 
 @[simp] theorem c_if_eq_te_evp:eval_prim O c_if_eq_te (Nat.pair (Nat.pair a b) (Nat.pair c d)) = if a=b then c else d := by
@@ -336,7 +367,8 @@ def c_if_lt_te :=
   c_add.comp₂
   (c_mul.comp₂ lt (right.comp right))
   (c_mul.comp₂ (c_not.comp lt) (left.comp right))
-@[simp, aesop safe] theorem c_if_lt_te_ev_pr:code_prim c_if_lt_te := by repeat (first|assumption|simp|constructor)
+@[cp] theorem c_if_lt_te_ev_pr:code_prim c_if_lt_te := by
+  repeat (first|assumption|apply_rules using cp|simp|constructor)
 @[simp] theorem c_if_lt_te_evp:eval_prim O c_if_lt_te (Nat.pair (Nat.pair a b) (Nat.pair c d)) = if a<b then c else d := by
   simp [c_if_lt_te,eval_prim];
   -- funext xs
@@ -360,7 +392,9 @@ namespace Nat.RecursiveIn.Code
 -- we use the fact that `a<b+1 ↔ a≤b`.
 /-- eval c_if_le_te (x,y) = [x≤y] -/
 def c_if_le_te := c_if_lt_te.comp (pair (pair (left.comp left) (succ.comp $ right.comp left)) right)
-@[simp, aesop safe] theorem c_if_le_te_ev_pr:code_prim c_if_le_te := by repeat (first|assumption|simp|constructor)
+@[cp] theorem c_if_le_te_ev_pr:code_prim c_if_le_te := by
+  unfold c_if_le_te
+  apply_rules (config := {maxDepth:=30, symm:=false, exfalso:=false, transparency:=.reducible}) only [*] using cp
 @[simp] theorem c_if_le_te_evp:eval_prim O c_if_le_te (Nat.pair (Nat.pair a b) (Nat.pair c d)) = if a≤b then c else d := by
   simp [c_if_le_te,eval_prim];
   -- funext xs
@@ -378,7 +412,9 @@ section flip
 namespace Nat.RecursiveIn.Code
 /-- eval c_flip (x,y) = (y,x) -/
 def c_flip := pair right left
-@[simp, aesop safe] theorem c_flip_ev_pr:code_prim c_flip := by repeat (first|assumption|simp|constructor)
+@[cp] theorem c_flip_ev_pr:code_prim c_flip := by
+  unfold c_flip
+  apply_rules (config := {maxDepth:=30, symm:=false, exfalso:=false, transparency:=.reducible}) only [*] using cp
 @[simp] theorem c_flip_evp:eval_prim O c_flip (Nat.pair a b) = Nat.pair b a := by
   simp [c_flip,eval_prim];
 @[simp] theorem c_flip_ev:eval O c_flip (Nat.pair a b) = Nat.pair b a := by
@@ -393,7 +429,9 @@ section if_gt_te
 namespace Nat.RecursiveIn.Code
 /-- eval c_if_gt_te (x,y) = [x>y] -/
 def c_if_gt_te := c_if_lt_te.comp (pair (c_flip.comp left) right)
-@[simp, aesop safe] theorem c_if_gt_te_ev_pr:code_prim c_if_gt_te := by repeat (first|assumption|simp|constructor)
+@[cp] theorem c_if_gt_te_ev_pr:code_prim c_if_gt_te := by
+  unfold c_if_gt_te
+  apply_rules (config := {maxDepth:=30, symm:=false, exfalso:=false, transparency:=.reducible}) only [*] using cp
 @[simp] theorem c_if_gt_te_evp:eval_prim O c_if_gt_te (Nat.pair (Nat.pair a b) (Nat.pair c d)) = if a>b then c else d := by simp [c_if_gt_te,eval_prim];
 @[simp] theorem c_if_gt_te_ev:eval O c_if_gt_te (Nat.pair (Nat.pair a b) (Nat.pair c d)) = if a>b then c else d := by
   rw [← eval_prim_eq_eval c_if_gt_te_ev_pr]; simp
@@ -405,7 +443,9 @@ section if_ge_te
 namespace Nat.RecursiveIn.Code
 /-- eval c_if_ge_te (x,y) = [x>y] -/
 def c_if_ge_te := c_if_le_te.comp (pair (c_flip.comp left) right)
-@[simp, aesop safe] theorem c_if_ge_te_ev_pr:code_prim c_if_ge_te := by repeat (first|assumption|simp|constructor)
+@[cp] theorem c_if_ge_te_ev_pr:code_prim c_if_ge_te := by
+  unfold c_if_ge_te
+  apply_rules (config := {maxDepth:=30, symm:=false, exfalso:=false, transparency:=.reducible}) only [*] using cp
 @[simp] theorem c_if_ge_te_evp:eval_prim O c_if_ge_te (Nat.pair (Nat.pair a b) (Nat.pair c d)) = if a≥b then c else d := by simp [c_if_ge_te,eval_prim];
 @[simp] theorem c_if_ge_te_ev:eval O c_if_ge_te (Nat.pair (Nat.pair a b) (Nat.pair c d)) = if a≥b then c else d := by
   rw [← eval_prim_eq_eval c_if_ge_te_ev_pr]; simp
@@ -417,7 +457,9 @@ end if_ge_te
 section ifz
 namespace Nat.RecursiveIn.Code
 def c_ifz := c_add.comp $ pair (c_mul.comp $ pair (c_sg'.comp left) (left.comp right)) (c_mul.comp $ pair (c_sg.comp left) (right.comp right))
-@[simp, aesop safe] theorem c_ifz_ev_pr:code_prim c_ifz := by repeat (first|assumption|simp|constructor)
+@[cp] theorem c_ifz_ev_pr:code_prim c_ifz := by
+  unfold c_ifz
+  apply_rules (config := {maxDepth:=30, symm:=false, exfalso:=false, transparency:=.reducible}) only [*] using cp
 @[simp] theorem c_ifz_evp:eval_prim O c_ifz = fun (cab:ℕ) => if cab.l=0 then cab.r.l else cab.r.r := by
   simp [c_ifz,eval_prim];
   funext xs
@@ -442,7 +484,9 @@ def c_nat_iterate (cf:Code) :=
   c_id
   (cf.comp (right.comp right))
 
-@[simp] theorem c_nat_iterate_ev_pr (hcf:code_prim cf) : code_prim (c_nat_iterate cf) := by repeat (first|assumption|simp|constructor)
+@[cp] theorem c_nat_iterate_ev_pr (hcf:code_prim cf) : code_prim (c_nat_iterate cf) := by
+  unfold c_nat_iterate
+  apply_rules (config := {maxDepth:=30, symm:=false, exfalso:=false, transparency:=.reducible}) only [*] using cp
 @[simp] theorem c_nat_iterate_evp : eval_prim O (c_nat_iterate cf) (Nat.pair input i) = (eval_prim O cf)^[i] (input) := by
   simp [c_nat_iterate]
   induction i with
@@ -462,7 +506,9 @@ end nat_iterate
 section mul2
 namespace Nat.RecursiveIn.Code
 def c_mul2 := c_mul.comp₂ c_id (c_const 2)
-@[simp] theorem c_mul2_ev_pr:code_prim c_mul2 := by repeat (first|assumption|simp|constructor)
+@[cp] theorem c_mul2_ev_pr:code_prim c_mul2 := by
+  unfold c_mul2
+  apply_rules (config := {maxDepth:=30, symm:=false, exfalso:=false, transparency:=.reducible}) only [*] using cp
 @[simp] theorem c_mul2_evp:eval_prim O c_mul2 = fun x => x*2 := by simp [c_mul2]
 @[simp] theorem c_mul2_ev:eval O c_mul2 = (fun x => x*(2:ℕ)) := by rw [← eval_prim_eq_eval c_mul2_ev_pr]; simp only [c_mul2_evp];
 end Nat.RecursiveIn.Code
@@ -474,64 +520,84 @@ end mul2
 
 namespace Nat.RecursiveIn.Code
 def c_zero := c_const zero
-@[simp, aesop safe] theorem c_zero_ev_pr:code_prim c_zero := by repeat (first|assumption|simp|constructor)
+@[cp] theorem c_zero_ev_pr:code_prim c_zero := by
+  unfold c_zero
+  apply_rules (config := {maxDepth:=30, symm:=false, exfalso:=false, transparency:=.reducible}) only [*] using cp
 @[simp] theorem c_zero_evp : eval_prim O c_zero x = encodeCode zero := by simp [c_zero]
 @[simp] theorem c_zero_evp' : eval_prim O c_zero = fun _:ℕ => encodeCode (zero) := by funext x; simp
 @[simp] theorem c_zero_ev:eval O c_zero x = encodeCode zero := by rw [← eval_prim_eq_eval c_zero_ev_pr]; simp
 @[simp] theorem Nat.PrimrecIn.c_zero : Nat.PrimrecIn O (fun _:ℕ => encodeCode zero) := by rw [←c_zero_evp']; exact code_prim_prop
 def c_succ := c_const succ
-@[simp, aesop safe] theorem c_succ_ev_pr:code_prim c_succ := by repeat (first|assumption|simp|constructor)
+@[cp] theorem c_succ_ev_pr:code_prim c_succ := by
+  unfold c_succ
+  apply_rules (config := {maxDepth:=30, symm:=false, exfalso:=false, transparency:=.reducible}) only [*] using cp
 @[simp] theorem c_succ_evp : eval_prim O c_succ x = encodeCode succ := by simp [c_succ]
 @[simp] theorem c_succ_evp' : eval_prim O c_succ = fun _:ℕ => encodeCode (succ) := by funext x; simp
 @[simp] theorem c_succ_ev:eval O c_succ x = encodeCode succ := by rw [← eval_prim_eq_eval c_succ_ev_pr]; simp
 @[simp] theorem Nat.PrimrecIn.c_succ : Nat.PrimrecIn O (fun _:ℕ => encodeCode succ) := by rw [←c_succ_evp']; exact code_prim_prop
 def c_left := c_const left
-@[simp, aesop safe] theorem c_left_ev_pr:code_prim c_left := by repeat (first|assumption|simp|constructor)
+@[cp] theorem c_left_ev_pr:code_prim c_left := by
+  unfold c_left
+  apply_rules (config := {maxDepth:=30, symm:=false, exfalso:=false, transparency:=.reducible}) only [*] using cp
 @[simp] theorem c_left_evp : eval_prim O c_left x = encodeCode left := by simp [c_left]
 @[simp] theorem c_left_evp' : eval_prim O c_left = fun _:ℕ => encodeCode (left) := by funext x; simp
 @[simp] theorem c_left_ev:eval O c_left x = encodeCode left := by rw [← eval_prim_eq_eval c_left_ev_pr]; simp
 @[simp] theorem Nat.PrimrecIn.c_left : Nat.PrimrecIn O (fun _:ℕ => encodeCode left) := by rw [←c_left_evp']; exact code_prim_prop
 def c_right := c_const right
-@[simp, aesop safe] theorem c_right_ev_pr:code_prim c_right := by repeat (first|assumption|simp|constructor)
+@[cp] theorem c_right_ev_pr:code_prim c_right := by
+  unfold c_right
+  apply_rules (config := {maxDepth:=30, symm:=false, exfalso:=false, transparency:=.reducible}) only [*] using cp
 @[simp] theorem c_right_evp : eval_prim O c_right x = encodeCode right := by simp [c_right]
 @[simp] theorem c_right_evp' : eval_prim O c_right = fun _:ℕ => encodeCode (right) := by funext x; simp
 @[simp] theorem c_right_ev:eval O c_right x = encodeCode right := by rw [← eval_prim_eq_eval c_right_ev_pr]; simp
 @[simp] theorem Nat.PrimrecIn.c_right : Nat.PrimrecIn O (fun _:ℕ => encodeCode right) := by rw [←c_right_evp']; exact code_prim_prop
 def c_oracle := c_const oracle
-@[simp, aesop safe] theorem c_oracle_ev_pr:code_prim c_oracle := by repeat (first|assumption|simp|constructor)
+@[cp] theorem c_oracle_ev_pr:code_prim c_oracle := by
+  unfold c_oracle
+  apply_rules (config := {maxDepth:=30, symm:=false, exfalso:=false, transparency:=.reducible}) only [*] using cp
 @[simp] theorem c_oracle_evp : eval_prim O c_oracle x = encodeCode oracle := by simp [c_oracle]
 @[simp] theorem c_oracle_evp' : eval_prim O c_oracle = fun _:ℕ => encodeCode (oracle) := by funext x; simp
 @[simp] theorem c_oracle_ev:eval O c_oracle x = encodeCode oracle := by rw [← eval_prim_eq_eval c_oracle_ev_pr]; simp
 @[simp] theorem Nat.PrimrecIn.c_oracle : Nat.PrimrecIn O (fun _:ℕ => encodeCode oracle) := by rw [←c_oracle_evp']; exact code_prim_prop
 
 def c_pair := c_add.comp₂ (c_mul2.comp $ c_mul2) (c_const 5)
-@[simp, aesop safe] theorem c_pair_ev_pr:code_prim c_pair := by repeat (first|assumption|simp|constructor)
+@[cp] theorem c_pair_ev_pr:code_prim c_pair := by
+  unfold c_pair
+  apply_rules (config := {maxDepth:=30, symm:=false, exfalso:=false, transparency:=.reducible}) only [*] using cp
 @[simp] theorem c_pair_evp : eval_prim O c_pair (Nat.pair a b) = encodeCode (pair a b) := by simp [encodeCode, c_pair, Nat.mul_comm]
 @[simp] theorem c_pair_evp' : eval_prim O c_pair = fun ab:ℕ => encodeCode (pair ab.l ab.r) := by simp [encodeCode, c_pair, Nat.mul_comm]
 @[simp] theorem c_pair_ev:eval O c_pair (Nat.pair a b) = encodeCode (pair a b) := by rw [← eval_prim_eq_eval c_pair_ev_pr]; simp
 @[simp] theorem Nat.PrimrecIn.c_pair : Nat.PrimrecIn O (fun ab:ℕ => encodeCode (pair ab.l ab.r)) := by rw [←c_pair_evp']; exact code_prim_prop
 
 def c_comp := c_add.comp₂ (c_mul2.comp $ c_mul2) (c_const 6)
-@[simp, aesop safe] theorem c_comp_ev_pr:code_prim c_comp := by repeat (first|assumption|simp|constructor)
+@[cp] theorem c_comp_ev_pr:code_prim c_comp := by
+  unfold c_comp
+  apply_rules (config := {maxDepth:=30, symm:=false, exfalso:=false, transparency:=.reducible}) only [*] using cp
 @[simp] theorem c_comp_evp : eval_prim O c_comp (Nat.pair a b) = encodeCode (comp a b) := by simp [encodeCode, c_comp, Nat.mul_comm]
 @[simp] theorem c_comp_evp' : eval_prim O c_comp = fun ab:ℕ => encodeCode (comp ab.l ab.r) := by simp [encodeCode, c_comp, Nat.mul_comm]
 @[simp] theorem c_comp_ev:eval O c_comp (Nat.pair a b) = encodeCode (comp a b) := by rw [← eval_prim_eq_eval c_comp_ev_pr]; simp
 @[simp] theorem Nat.PrimrecIn.c_comp : Nat.PrimrecIn O (fun ab:ℕ => encodeCode (comp ab.l ab.r)) := by rw [←c_comp_evp']; exact code_prim_prop
 
 def c_prec := c_add.comp₂ (c_mul2.comp $ c_mul2) (c_const 7)
-@[simp, aesop safe] theorem c_prec_ev_pr:code_prim c_prec := by repeat (first|assumption|simp|constructor)
+@[cp] theorem c_prec_ev_pr:code_prim c_prec := by
+  unfold c_prec
+  apply_rules (config := {maxDepth:=30, symm:=false, exfalso:=false, transparency:=.reducible}) only [*] using cp
 @[simp] theorem c_prec_evp : eval_prim O c_prec (Nat.pair a b) = encodeCode (prec a b) := by simp [encodeCode, c_prec, Nat.mul_comm]; exact rfl
 @[simp] theorem c_prec_evp' : eval_prim O c_prec = fun ab:ℕ => encodeCode (prec ab.l ab.r) := by simp [encodeCode, c_prec, Nat.mul_comm]; exact rfl
 @[simp] theorem Nat.PrimrecIn.c_prec : Nat.PrimrecIn O (fun ab:ℕ => encodeCode (prec ab.l ab.r)) := by rw [←c_prec_evp']; exact code_prim_prop
 @[simp] theorem c_prec_ev:eval O c_prec (Nat.pair a b) = encodeCode (prec a b) := by rw [← eval_prim_eq_eval c_prec_ev_pr]; simp
 
 def c_rfind' := c_add.comp₂ (c_mul2.comp $ c_mul2) (c_const 8)
-@[simp, aesop safe] theorem c_rfind'_ev_pr:code_prim c_rfind' := by repeat (first|assumption|simp|constructor)
+@[cp] theorem c_rfind'_ev_pr:code_prim c_rfind' := by
+  unfold c_rfind'
+  apply_rules (config := {maxDepth:=30, symm:=false, exfalso:=false, transparency:=.reducible}) only [*] using cp
 @[simp] theorem c_rfind'_evp : eval_prim O c_rfind' c = encodeCode (rfind' c) := by simp [encodeCode, c_rfind', Nat.mul_comm]; exact rfl
 @[simp] theorem c_rfind'_ev:eval O c_rfind' c = encodeCode (rfind' c) := by rw [← eval_prim_eq_eval c_rfind'_ev_pr]; simp
 
 def c_c_const := (c_nat_iterate (c_comp.comp₂ (c_const succ) (c_id))).comp₂ zero c_id
-@[simp, aesop safe] theorem c_c_const_ev_pr:code_prim c_c_const := by repeat (first|assumption|simp|constructor)
+@[cp] theorem c_c_const_ev_pr:code_prim c_c_const := by
+  unfold c_c_const
+  apply_rules (config := {maxDepth:=30, symm:=false, exfalso:=false, transparency:=.reducible}) only [*] using cp
 @[simp] theorem c_c_const_evp : eval_prim O c_c_const n = encodeCode (c_const n) := by
   unfold c_const
   unfold c_c_const
@@ -552,7 +618,9 @@ theorem c_c_const_evp' : eval_prim O c_c_const = c_const := by
 @[simp] theorem Nat.PrimrecIn.c_const:Nat.PrimrecIn O c_const := by rw [← c_c_const_evp']; exact code_prim_prop
 
 def c_ev_const := c_comp.comp₂ left (c_c_const.comp right)
-@[simp, aesop safe] theorem c_ev_const_ev_pr:code_prim c_ev_const := by repeat (first|assumption|simp|constructor)
+@[cp] theorem c_ev_const_ev_pr:code_prim c_ev_const := by
+  unfold c_ev_const
+  apply_rules (config := {maxDepth:=30, symm:=false, exfalso:=false, transparency:=.reducible}) only [*] using cp
 theorem c_ev_const_evp' : eval_prim O c_ev_const x = encodeCode (comp x.l (c_const x.r)) := by simp [c_ev_const]
 @[simp] theorem c_ev_const_evp : eval_prim O c_ev_const (Nat.pair e x) = encodeCode (comp e (c_const x)) := by simp [c_ev_const_evp']
 theorem c_ev_const_ev':eval O c_ev_const x = encodeCode (comp x.l (c_const x.r)) := by rw [← eval_prim_eq_eval c_ev_const_ev_pr]; simp [c_ev_const_evp']
@@ -562,7 +630,9 @@ end Nat.RecursiveIn.Code
 section max
 namespace Nat.RecursiveIn.Code
 def c_max := c_if_le_te.comp₄ left right right left
-@[simp, aesop safe] theorem c_max_ev_pr:code_prim c_max := by repeat (first|assumption|simp|constructor)
+@[cp] theorem c_max_ev_pr:code_prim c_max := by
+  unfold c_max
+  apply_rules (config := {maxDepth:=30, symm:=false, exfalso:=false, transparency:=.reducible}) only [*] using cp
 @[simp] theorem c_max_evp:eval_prim O c_max = unpaired2 Nat.max := by
   simp [c_max,eval_prim, -pair_lr]
   exact rfl
